galois/network/action.lean
@@ -7,92 +7,17 @@ universes u v
 namespace network
 
 inductive act (A : Type u) : Type u
-| return : A → act
-| connect : remote_name → (socket → act) → act
-| send_message : socket -> message_t → act → act
+--| connect : remote_name → (socket → A) → act
 -- return a poll result and the amount of time elapsed
 | poll : Π (ports : list port) (sockets : list socket) (bound : time), 
-     (poll_result ports sockets bound → act) → act
+     (poll_result ports sockets bound → (list (socket × message_t) × A)) → act
 
-def act_bind {A B : Type u} (x : act A) (f : A → act B) : act B
-:= begin
-induction x,
-{ apply f, assumption },
-{ apply act.connect; assumption },
-{ apply act.send_message; assumption },
-{ apply act.poll; try {assumption} }
-end
+namespace act
+def just_send_messages {A : Type u} (ms : list (socket × message_t)) 
+  (x : A) := act.poll [] [] 0 (λ _, (ms, x))
 
-lemma act_bind_pure {α : Type u} (x : act α)
-: act_bind x act.return = x :=
-begin
-  simp [act_bind], induction x; dsimp,
-  { reflexivity },
-  { dsimp at ih_1,  
-    apply congr_arg, apply funext,
-    intros s, apply ih_1 },
-  { apply congr_arg, apply ih_1 },
-  { dsimp at ih_1,
-    apply congr_arg, apply funext,
-    intros t, apply ih_1 }
-end
-
-instance act_is_monad : monad act :=
-{ pure := @act.return
-, bind := @act_bind
-, id_map := begin intros, dsimp, apply act_bind_pure end
-, pure_bind :=
-begin
-  intros, simp [act_bind],
-end
-, bind_assoc :=
-begin
-  intros, induction x,
-  { reflexivity },
-  { simp [act_bind], dsimp,
-    apply congr_arg, apply funext,
-    intros s, apply ih_1 },
-  { simp [act_bind],
-    apply congr_arg, apply ih_1 },
-  { simp [act_bind], dsimp,
-    apply congr_arg, apply funext,
-    intros s, apply ih_1 }
-end
-}
-
-instance act_is_network_monad : network_monad act :=
-  { to_monad := network.act_is_monad
-  , socket := remote_name
-  , connect := λ x, act.connect x act.return
-  , send := λ x y, act.send_message x y (act.return punit.star)
-  , poll := λ x y z, act.poll x y z act.return  
-  }
-
-lemma act_bind_poll {A : Type} {ports sockets bound}
-  (f : poll_result ports sockets bound → act A)
-  : poll ports sockets bound >>= f
-  = act.poll ports sockets bound f
-:= rfl
-
-lemma act_bind_send {B : Type} {rn : remote_name}
-  {mess : message_t}
-  (f : act B)
-  : @send _ network.act_is_network_monad rn mess >> f 
-    = act.send_message rn mess f
-  := rfl
-
-lemma act_bind_connect {B : Type} {rn : remote_name}
-  (f : socket → act B)
-  : @network_monad.connect _ network.act_is_network_monad rn >>= f 
-    = act.connect rn f
-  := rfl
-
-lemma act_bind_return {A B : Type} {x : A}
-  (f : A → act B)
-  : return x >>= f 
-    = f x
-  := rfl
-    
+def return {A : Type u} (x : A) : act A := just_send_messages [] x
+end act
 
 -- An agent is defined as a type for the internal state, an process that produces
 -- the state, and a looping process that will execute when the process is complete.
@@ -116,11 +41,8 @@ inductive poll_dlabel (ports : list port) (sockets : list socket) (bound : ℕ) 
     → poll_dlabel
 
 inductive dlabel : act ag.state_type → Type
-| update_own_state : ∀ new_state : ag.state_type, dlabel (act.return new_state)
-| connect : ∀ (rn : remote_name) cont, dlabel (act.connect rn cont)
-| send_message : ∀ sock mess cont,
-      dlabel (act.send_message sock mess cont)
-| poll : ∀ (ports : list port) (sockets : list socket) (bound : time) cont,
+| poll : ∀ (ports : list port) (sockets : list socket) (bound : time) 
+    cont (ms : list (socket × message_t)),
     poll_dlabel ports sockets bound
     → dlabel (act.poll ports sockets bound cont)
 
