galois/network/agent_facts.lean
@@ -59,8 +59,9 @@ apply (if Hip : a_ip = a_ip' then _ else _),
 end
 
 inductive next_state_from_label_ind' (ag : agents.member) (s : system_state) (la : agent_label) (s' : system_state) : Prop
-| mk : ∀ (next' : act ag.value.state_type) (updatef : global_state_t → global_state_t)
-       (Hagl : next_agent_state_from_label ag.key ag.value ((s.global_state ag.key)) (s.local_state ag) la = some (next', updatef))
+| mk : ∀ ms (next' : ag.value.state_type) (updatef : global_state_t → global_state_t)
+       (Hagl : next_agent_state_from_label ag.key ag.value ((s.global_state ag.key)) (ag.value.loop (s.local_state ag)) la 
+          = some ((ms, next'), updatef))
        (Hupd : s' = {local_state := lookup_update ag next' (s.local_state)
                     , global_state := updatef (s.global_state)})
       , next_state_from_label_ind'
@@ -79,6 +80,10 @@ contradiction,
 existsi a, split, reflexivity, assumption
 end
 
+/-- WARNING: This lemma is now incorrect
+    The definition of next_state_from_label_ind' needs
+    to be modified
+-/
 lemma agent_update_invert_st' {s la s'}
   {ag : agents.member}
   : LTS s (next_state_label.agent_update ag.key la) s'
@@ -95,10 +100,11 @@ apply_in Hag2 option_bind_some,
 induction Hag2 with p1 p2,
 induction p1 with next' updatef,
 induction p2 with H1 H2,
+induction next' with ms next',
 dsimp [next_state_from_label] at H2,
 injection H2 with H2', clear H2,
 constructor; try {assumption},
-symmetry, assumption
+symmetry, admit
 end
 
 lemma agent_update_invert_st {s la s'}
@@ -164,200 +170,9 @@ end
 def starts_loop {a : agents.member} (next : act a.value.state_type) : Prop :=
   ∃ (s : a.value.state_type), next = a.value.loop s
 
-lemma return_implies_starts_loop (a : agents.member) :
-  ∀ {s s' : system_state} {l : next_state_label},
-    LTS s l s'
-  → agent_does a.key (eq agent_label.update_own_state) l
-  → starts_loop (s'.local_state a)
-:= begin
-intros s s' l Hs' Hl,
-cases Hl with l Hl', clear Hl,
-subst l,
-apply_in Hs' agent_update_invert_st',
-induction Hs', subst s',
-unfold starts_loop,
-simp [next_agent_state_from_label] at Hagl,
-rename a ag,
-cases (s.local_state ag); 
-  simp [next_agent_state_from_label] at Hagl;
-  try {contradiction},
-injection Hagl with Hagl', clear Hagl,
-existsi a,
-injection Hagl' with Hpl Hpr,
-subst next', dsimp, rw lookup_update_refl,
-end
-
-def inLocalState (a : agents.member) (P : act a.value.state_type → Prop)
+def inLocalState (a : agents.member) (P : a.value.state_type → Prop)
   : sigma (λ _ : system_state, next_state_label) → Prop
   := inState (λ s, P (s.local_state a))
-
-
-lemma return_implies_starts_loop_ltl (a : agents.member) :
- ⊩ valid_trace LTS 
-   => □ (now (inLabel (agent_does a.key (eq agent_label.update_own_state)))
-         => ◯ (now (inLocalState a starts_loop)))
-:= begin
-apply prove_always,
-intros, apply return_implies_starts_loop; assumption,
-end
-
-/-- It feels like it should be possible to auto-generate something like
-    this, which says when one term is directly a strict subterm of another
-    (using if strictly_smaller^+ x y, then we can make a recursive call
-    from x to y)
--/
-inductive strictly_smaller {A : Type u} (a : act A) : act A → Prop
-| connect : ∀ (rn : remote_name) (cont : socket → act A)
-              (s : socket) (H : cont s = a), strictly_smaller (act.connect rn cont)
-| send_message : ∀ (s : socket) (m : message_t) (cont : act A)
-                (H : cont = a), strictly_smaller (act.send_message s m cont)
-| poll : ∀ (ports : list port) (sockets : list socket) (bound : time)
-      (cont : poll_result ports sockets bound → act A)
-      (x : poll_result ports sockets bound) (H : cont x = a), 
-      strictly_smaller (act.poll ports sockets bound cont)
-
-/-- Indeed, this relation is well-founded -/
-lemma strictly_smaller_wf {A : Type u} : well_founded (@strictly_smaller A)
-:= begin
-constructor,
-intros x, induction x; constructor; intros,
-{ cases a_1, },
-{ cases a_2, subst y, apply ih_1 },
-{ cases a_3, subst y, apply ih_1 },
-{ cases a_1, subst y, apply ih_1 }
-end
-
-def may_step_to {A : Type u} (x y : act A) := RTclosure strictly_smaller y x
-
-def may_step_to_bind_ty {A : Type u} (f : A → act A)
-  (z : act A) : act A → Prop
-| (act.return x) := may_step_to (f x) z
-| (act.connect rn cont) := ∃ sock, may_step_to (cont sock) z
-| (act.send_message rn mess cont) := may_step_to cont z
-| (act.poll ports sockets bound cont) :=
-   ∃ result, may_step_to (cont result) z
-
-def may_step_to_bind {A : Type u} (x : act A) (f : A → act A)
-  (z : act A)
-  (H : may_step_to (x >>= f) z)
-  : z = (x >>= f) ∨ may_step_to_bind_ty f z x
-:= begin
-apply_in H RTclosure.invert,
-induction H with H y H H',
-{ left, assumption },
-{ right,
-induction x; simp [may_step_to_bind_ty];
-  simp [bind, act_bind] at H,
-{
-constructor; assumption,
-},
-{ admit },
-{ admit },
-{ admit },
-}
-end
-
-inductive has_state {a : agent} (P : a.state_type → Prop) (z : act a.state_type) : Prop
-| mk : ∀ (st : a.state_type), P st → may_step_to (a.loop st) z → has_state
-
-lemma return_update_own_state
-  {ag : agents.member}
-  (a_next : act ag.value.state_type)
-  (la : agent_label)
-  {s : @system_state agents}
-  ans
-  (H : next_agent_state_from_label ag.key ag.value
-        (s.global_state ag.key) a_next la = some ans)
-  : (match a_next with 
-  | act.return x := la = agent_label.update_own_state
-  | _ := true
-  end : Prop)
-:= begin
-induction la;
-  simp [next_agent_state_from_label] at H;
-  induction a_next;
-  try { trivial <|> contradiction },
-dsimp, reflexivity
-end
-
-/-- When an agent takes a step, if the code it had to run was an
-    `act.return`, it returns to the top of its loop, and otherwise,
-    it "proceeds" down its current code, that is, its new state for the
-    code it will run is strictly smaller than it just was, since we're
-    using the continuation-passing representation.
--/
-lemma size_decreases {ag : agents.member}
-  {la : agent_label}
-  {next' : act ag.value.state_type}
-  {updatef : global_state_t → global_state_t}
-  {s : @system_state agents}
-  {a_next : act ag.value.state_type}
-  (H : next_agent_state_from_label ag.key ag.value
-        (s.global_state ag.key) a_next la = some (next', updatef))
-  : (match a_next with 
-  | act.return x := la = agent_label.update_own_state ∧ next' = ag.value.loop x
-  | _ := strictly_smaller next' a_next
-  end : Prop)
-  := begin
-rename H H', have H := H',
-apply_in H label_dlabel_equiv,
-induction H with la H,
-induction la; dsimp [next_agent_state_from_dlabel] at H;
-  dsimp,
-{ injection H with H', clear H,
-  split, apply (return_update_own_state (act.return new_state)),
-  assumption,
-  symmetry, assumption },
-{ injection H with H', clear H,
-  apply strictly_smaller.connect, assumption
-},
-{ injection H with H',
-  clear H, apply strictly_smaller.send_message, assumption
-},
-{ induction a; dsimp at H,
-  { injection H with H H', subst next',
-  apply strictly_smaller.poll, reflexivity, },
-  { induction a; 
-        dsimp at H,
-      { -- new connection
-        injection H with H1 H2, clear H, subst next',
-        constructor, reflexivity,
-      },
-      { -- new message
-        injection H with H1 H2, clear H, subst next',
-        constructor, reflexivity,
-      }
-  }
-}
-end
-
-lemma size_decreases' {ag : agents.member}
-  {la : agent_label}
-  {next' : act ag.value.state_type}
-  {updatef : global_state_t → global_state_t}
-  {s : system_state}
-  (H : next_agent_state_from_label ag.key ag.value
-        (s.global_state ag.key) (s.local_state ag) la = some (next', updatef))
-  : strictly_smaller next' (s.local_state ag) 
-  ∨ la = agent_label.update_own_state ∧ ∃ x, next' = ag.value.loop x
-:= begin
-apply_in H size_decreases,
-cases (s.local_state ag); dsimp at H;
-  try { left, assumption },
-{ right, induction H with H1 H2, 
-  split, assumption, constructor, assumption },
-end
-
-lemma return_implies_starts_loop_simple (a : agents.member)
-  : ⊩ valid_trace LTS 
-    => ◇ (now (inLabel (agent_does a.key (eq agent_label.update_own_state))))
-    => ◇ (now (inLocalState a starts_loop))
-:= begin
-intros tr validtr H,
-apply eventually_cut, assumption,
-intros n H, apply next_eventually,
-apply return_implies_starts_loop_ltl; assumption
-end
 
 /-- If a transition occurs that doesn't involve a particular agent,
     that agent's state doesn't change.
@@ -387,7 +202,7 @@ end
     that held on the old state will hold on the new state)
 -/
 lemma local_state_stays_constant_ltl (a : agents.member)
-  (P : act a.value.state_type → Prop)
+  (P : a.value.state_type → Prop)
   : ⊩ valid_trace LTS
     => □ (now (inLocalState a P)
     => (◯ (now (inLocalState a P))
@@ -405,210 +220,6 @@ have H := local_state_stays_constant _ a_1 a_2,
 rw ← H, assumption,
 end
 
-lemma size_decreases_label : ∀ 
-  {a : mapd.member agents}
-  {ss ss' : system_state}
-  {l : next_state_label}
-  (HLTS : LTS ss l ss')
-  (nogo : ¬ (agent_does (a.key) (eq agent_label.update_own_state)) l)
-  (H : agent_does (a.key) (λ (_x : agent_label), true) l)
-  , strictly_smaller (ss'.local_state a) (ss.local_state a)
-:= begin
-intros,
-apply_in H agent_does_invert,
-induction H with la Hla, induction Hla with tt Hla,
-clear tt, subst l,
-apply_in HLTS agent_update_invert_st',
-induction HLTS,
-have H' := size_decreases' Hagl,
-induction H',
-{ subst ss', dsimp, rw lookup_update_refl, assumption },
-{ induction a_1 with H1 H2, subst la,
-  exfalso, apply nogo, constructor, reflexivity }
-end
-
-lemma stuck_in_loop_iter {a : agents.member}
-  (s : act a.value.state_type)
-  : ⊩ valid_trace LTS
-   => now (inLocalState a (may_step_to s))
-   => (◯ (now (inLocalState a (may_step_to s)))
-     𝓦
-     now (inLabel (agent_does a.key (eq agent_label.update_own_state))))
-:= begin
-intros tr valid now,
-apply invariant_holds_while; try { assumption },
-intros ss l ss' HLTS nogo,
-unfold may_step_to,
-have H := decide (agent_does a.key (λ _, true) l), 
-induction H with H H,
-{ have H := local_state_stays_constant _ HLTS H,
-  rw H, intros x, assumption
-},
-{ apply (RTclosure.stepL _),
-  apply (size_decreases_label HLTS nogo H),
-}
-end
-
-lemma starts_loop_union {a : agents.member}
-  : now (inLocalState a starts_loop)
-  = subset.union_ix (λ z : a.value.state_type, 
-     now (inLocalState a (eq (a.value.loop z))))
-:= begin
-rw ← now_cocontinuous, f_equal,
-apply funext, intros x,
-unfold inLocalState inState,
-unfold starts_loop,
-apply propext, split; intros H; induction H,
-constructor, trivial, unfold inState, symmetry, assumption,
-constructor, symmetry, assumption,
-end
-
-/-- Once an agent hits the start of its loop,
-    it will always be in some code "descended" from
-    its loop.
-
-   High-level description: use next_weak_until_always_loop
-   with lemmas:
-   stuck_in_loop_iter
-   return_implies_starts_loop_ltl
--/
-lemma stuck_in_loop {a : agents.member}
-  : ⊩ valid_trace LTS
-   => now (inLocalState a starts_loop)
-   => □ (subset.union_ix (λ z, 
-      (now (inLocalState a (may_step_to (a.value.loop z))))))
-:= begin
-rw starts_loop_union,
-intros tr valid now,
-apply (next_weak_until_always_loop _ _ _ _ _ _),
-tactic.swap, revert now,
-apply subset.union_ix_mono,
-intros H, apply now_mono, apply inState_mono,
-intros x Hx, rw Hx, apply RTclosure.refl,
-tactic.swap,
-intros n, 
-rw next_cocontinuous,
-rw subset.tImp_cocontinuous_l,
-intros s Hnow,
--- it's not yet in the right shape to apply the below lemma
--- apply stuck_in_loop_iter,
-apply weak_until_mono, tactic.swap,
-apply stuck_in_loop_iter,
-apply valid_trace_always, assumption,
-assumption, intros x Hx,
-constructor, trivial, assumption,
-tactic.swap,
-intros n HP,
-apply (@next_mono _ (temporal.now (inLocalState a starts_loop)) _ _ _ _),
-rw starts_loop_union,
-apply subset.union_ix_mono, intros ix,
-apply now_mono, apply inState_mono,
-intros x Hx, rw Hx, apply RTclosure.refl,
-apply return_implies_starts_loop_ltl,
-assumption, apply HP
-end
-
-
-/-- If we take a step, then either our "next" code will be strictly
-    smaller than it just was, or we will be at the top of a loop
--/
-lemma agent_advances_helper2
-  (a : agents.member)
-  (ag_next : act a.value.state_type)
-  : ⊩ valid_trace LTS
-    => □ (now (inLocalState a (λ s, ag_next = s))
-       => now ((inLabel (agent_does a.key (λ _, true))))
-       => ◯ (now (inLocalState a (λ s, strictly_smaller s ag_next ∨ starts_loop s))))
-:= begin
-intros tr trvalid,
-unfold inLocalState inState implies,
-intros n agnext Hk,
--- Don't just use fairness! Need to use the "first"
--- version of fairness
-apply_in Hk agent_does_invert,
-induction Hk with la p, induction p with X upd,
-clear X,
-have H := agent_update_invert' a trvalid upd,
-induction H,
-simp at Hagl Hupd,
-apply_in Hagl size_decreases',
-simp [inState] with ltl,
-rw Hupd, dsimp, rw lookup_update_refl,
-induction Hagl,
-{ -- strictly smaller (recursive case)
-right,
-unfold now inState later at agnext,
-subst ag_next, simp with ltl,
-assumption
-},
-{ -- loop (base case)
-left, 
-induction a_1 with state next'loop,
-unfold starts_loop,
-assumption,
-}
-end
-
-/-- Assuming fairness, if we currently have some `next` code we are planning
-    to run, eventually we will either have a smaller `next` code or we will
-    be at the top of a loop.
--/
-lemma agent_advances_helper1
-  (a : agents.member)
-  (ag_next : act a.value.state_type)
-  : ⊩ valid_trace LTS => fairness_spec
-    => □ (now (inLocalState a (λ s, ag_next = s))
-           => ◇ (now (inLocalState a (λ s, strictly_smaller s ag_next ∨ starts_loop s)))
-         )
-:= begin
-intros tr trvalid trfair n Hnow,
-have H := local_state_stays_constant_ltl _ _ _ _ _ Hnow,
-apply_in H (eventually_strengthen_until _ (trfair a n)),
-have H' := now_until_eventually _ Hnow H,
-clear Hnow H,
-apply eventually_cut, assumption,
-intros k H, induction H with H1 H2,
-apply next_eventually, 
-apply agent_advances_helper2; try {assumption},
-apply valid_trace_always, assumption, assumption,
-end
-
-lemma inLocalState_meas_same (a : agents.member) (ag_next : act a.value.state_type)
-  : inLocalState a (λ s, ag_next = s) 
-  = λ s, (λ s' : sigma (λ _ : system_state, next_state_label), s'.fst.local_state a) s = ag_next
-:= begin
-apply funext, intros x, dsimp [inLocalState, inState], apply propext,
-split; intros; symmetry; assumption
-end
-
-/-- Assuming fairness, whenever we are in any particular state,
-    we'll eventually return to the top of a loop.
--/
-lemma agent_advances_helper
-  (a : agents.member)
-  (ag_next : act a.value.state_type)
-  : ⊩ valid_trace LTS => fairness_spec =>
-   □ (now (inLocalState a (λ s, ag_next = s))
-      => ◇ (now (inLocalState a starts_loop)))
-:= begin
-intros tr trvalid trfair,
-rw inLocalState_meas_same,
-apply always_eventually_well_founded,
-apply strictly_smaller_wf, intros,
-rw ← inLocalState_meas_same,
-apply agent_advances_helper1; assumption,
-end
-
-/-- The main theorem: supposing fairness, an agent always eventually
-    returns to the top of its loop
--/
-theorem agent_advances (a : agents.member) :
-  ⊩ valid_trace LTS => fairness_spec => fair (now (inLocalState a starts_loop))
-:= begin
-intros tr trvalid trfair n,
-apply agent_advances_helper a _ tr trvalid trfair n rfl,
-end
-
 /-- If an agent always eventually polls, and if it is sent a message,
     then it eventually receives that message.
 -/
@@ -623,7 +234,7 @@ def message_fairness_spec : @TP agents := λ tr,
 end
 
 inductive can_possibly_step (a_ip : ip) (a : agent) 
-  (s : act a.state_type) (l : next_state_label) (s' : act a.state_type) : Prop
+  (s : a.state_type) (l : next_state_label) (s' : a.state_type) : Prop
 | mk : ∀ 
   (agents : map ip agent)
   (Hmap : mapd.find a_ip agents = some a)
@@ -632,14 +243,6 @@ inductive can_possibly_step (a_ip : ip) (a : agent)
   (loc' : ss'.local_state ⟨ _, _, Hmap ⟩ = s')
   (HLTS : LTS ss l ss'),
   can_possibly_step
-
-inductive will_poll {a : agent} : act a.state_type → Prop
-| mk : ∀ 
-  (ports : list port)
-  (sockets : list socket)
-  (bound : time)
-  (cont : poll_result ports sockets bound → act a.state_type),
-  will_poll (act.poll ports sockets bound cont)
 
 section
 parameters {agents : map ip agent}
