galois/network/labels.lean
@@ -29,10 +29,7 @@ instance poll_label_decidable_eq
   := by tactic.mk_dec_eq_instance
 
 inductive agent_label : Type
-  | update_own_state : agent_label
-  | connect : remote_name → agent_label
-  | send_message : remote_name → message_t → agent_label
-  | poll : poll_label → agent_label
+  | poll : poll_label → list (remote_name × message_t) → agent_label
 
 /-- Decidable equality is straightforward, but currently it's
     difficult for me to automate.
@@ -49,7 +46,7 @@ inductive agent_does (a : ip) (P : agent_label → Prop) : next_state_label → 
 
 /-- Indicates that an agent is polling -/
 inductive polls : agent_label → Prop
-| mk : ∀ (l : poll_label), polls (agent_label.poll l)
+| mk : ∀ (l : poll_label) ms, polls (agent_label.poll l ms)
 
 instance polls_decidable : decidable_pred polls
 := begin
@@ -59,12 +56,12 @@ apply decidable.is_true, constructor,
 end
 
 inductive receives (P : poll_receive_label → Prop) : agent_label → Prop
-| mk : ∀ (t : time) (rn : remote_name) (prl : poll_receive_label),
-       P prl → receives (agent_label.poll (poll_label.receive t rn prl))
+| mk : ∀ (t : time) (rn : remote_name) (prl : poll_receive_label) ms,
+       P prl → receives (agent_label.poll (poll_label.receive t rn prl) ms)
 
 inductive receives_or_timeout (P : poll_receive_label → Prop) (l : agent_label) : Prop
 | receives : receives P l → receives_or_timeout
-| timeouts : l = agent_label.poll poll_label.timeout -> receives_or_timeout
+| timeouts : ∀ ms, l = agent_label.poll poll_label.timeout ms -> receives_or_timeout
 
 def receives_message (m : message_t) : agent_label → Prop :=
   receives (eq (poll_receive_label.receive_message m))
