galois/network/network_local_abs.lean
@@ -20,47 +20,41 @@ parameters (a_ip : ip) (ag : agent)
 
 def next_receive_dlabel {ports : list port} {sockets : list socket}
   {bound : time}
-  (cont : poll_result ports sockets bound → act ag.state_type)
+  (cont : poll_result ports sockets bound → list (socket × message_t) × ag.state_type)
   (elapsed_fin : fin bound) (rn : remote_name)
   : poll_receive_dlabel_abs ports sockets
-  → act ag.state_type
+  → list (socket × message_t) × ag.state_type
 | (poll_receive_dlabel_abs.new_connection p sock) :=
      cont (poll_result.new_connection elapsed_fin p sock)
 | (poll_receive_dlabel_abs.receive_message sock mess) := 
      cont (poll_result.message elapsed_fin sock mess)
 
 def next_poll_dlabel {ports : list port} {sockets : list socket}
-  {bound : time} (cont : poll_result ports sockets bound → act ag.state_type)
+  {bound : time} (cont : poll_result ports sockets bound → list (socket × message_t) × ag.state_type)
   : @poll_dlabel poll_receive_dlabel_abs ports sockets bound 
-  → act ag.state_type
+  → list (socket × message_t) × ag.state_type
 | poll_dlabel.timeout := cont poll_result.timeout
 | (poll_dlabel.receive elapsed_fin rn rlabel) := next_receive_dlabel
      cont elapsed_fin rn rlabel
 
 def next_agent_state_from_dlabel
   : ∀ (a_next : act ag.state_type) (la : dlabel' a_next)
-  , act ag.state_type
-| (act.return new_state) (dlabel.update_own_state ._) := ag.loop new_state
-| (act.connect rn cont) (dlabel.connect ._ ._) := cont rn
-| (act.send_message sock mess cont) (dlabel.send_message ._ ._ ._) := cont
-| (act.poll ports sockets bound cont) (dlabel.poll ._ ._ ._ ._ plabel)
-    := next_poll_dlabel cont plabel
+  , ag.state_type
+| (act.poll ports sockets bound cont) (dlabel.poll ._ ._ ._ ._ ms plabel)
+    := (next_poll_dlabel cont plabel).snd
 
 inductive sends_message_st (P : socket → message_t → Prop) : act ag.state_type → Prop
-| mk : ∀ sock mess cont, P sock mess 
-     → sends_message_st (act.send_message sock mess cont)
+| mk : ∀ ports sockets bound sock mess 
+    (cont : poll_result ports sockets bound →  list (socket × message_t) × ag.state_type)
+     , P sock mess
+     → (∀ res : poll_result ports sockets bound, (sock, mess) ∈ (cont res).fst)
+     → sends_message_st (act.poll ports sockets bound cont)
 
 instance sends_message_st_decidable (P : socket → message_t → Prop) 
   [decP : ∀ x y, decidable (P x y)] : decidable_pred (sends_message_st P)
 := begin
-intros x, induction x;
-  try { solve1 {apply decidable.is_false, intros x, cases x} },
-have H := decP a a_1, induction H,
-{ apply decidable.is_false, intros contra, cases contra,
-  apply a_3, assumption },
-{ apply decidable.is_true, 
-  constructor, assumption
-}
+intros x, induction x,
+admit
 end
 
 def LTS s l s' := next_agent_state_from_dlabel s l = s'
